much cleaning; simplify proofs a lot

Project.v
@@ -1,16 +1,19 @@
 
-Require Import Arith.
+(** * Stratified System F - Part I *)
 
-Require Import Le.
-Require Import Lt.
-Require Import Gt.
-Require Import Decidable.
+Require Import Arith.
 Require Import Max.
+Require Import Decidable.
 Require Import NPeano.
-Require Import GenericMinMax.
 Require Import Bool.
 Require Import Omega.
+Require Import Psatz.
+Require Import List.
+Require Import Relation_Definitions.
+Require Import Relation_Operators.
+Import ListNotations.
 Local Open Scope nat_scope.
+Local Open Scope bool_scope.
 
 (** ** 1.2 Definitions *)
 (** *** Question 1: Types *)
@@ -21,56 +24,60 @@ Inductive typ :=
 | fall : nat -> typ -> typ. (**r [nat] is the kind of the type which is abstracted. *)
 
 (** The environment is a stack of values.                                   *)
-(** If a term has v bounded variables then they are reprensented by
-    de Brujin indexes 0..v-1. From index v and on, the de Brujin indexes
+(** If a term has [v] bounded variables then they are reprensented by
+    de Bruijn indices [0..v-1]. From index [v] and on, the de Bruijn indices
     represent the free variables - that must appear in the environment then -
-    v being the top of the stack                                            *)
+    [v] being the top of the stack                                           *)
 
 (** The following function shifts the free type variables
-    by one within the type t.                             *)
-(** v is the number of bounded variables
-    - ie number of type abstractions - in t.              *)
+    by one within the type [t].                           *)
+(** [v] is the number of bounded variables
+    - ie number of lambda abstractions around [t].        *)
 Fixpoint tshift (t:typ) (v:nat) : typ := 
   match t with
-    | vart i   =>  vart (if le_gt_dec v i then 1 + i else i  )
+    | vart i   =>  vart (if le_gt_dec v i then 1 + i else i)
     | arrow t1 t2  => arrow (tshift t1 v) (tshift t2 v) 
     | fall rank sP  => fall rank (tshift sP (1 + v)) 
   end.
 
-Lemma tshift_lemma_1 :
+(** The following lemma was inspired by Vouillon also we changed
+    the proof a lot. It will be useful in the next section.      *)
+Lemma tshift_lemma :
   forall (T : typ) (X Y : nat),
     tshift (tshift T X) (S (X + Y)) = tshift (tshift T (X + Y)) X.
 Proof.
   induction T; intros X Y.
   + unfold tshift.
     destruct (le_gt_dec (S (X + Y)));
-      destruct (le_gt_dec (X + Y) n);
-      destruct (le_gt_dec X n);
-      destruct (le_gt_dec X (1 + n)); trivial; omega.
+    destruct (le_gt_dec (X + Y) n);
+    destruct (le_gt_dec X n);
+    destruct (le_gt_dec X (1 + n)); trivial; omega.
   + apply f_equal2 with (f := arrow); trivial.
   + simpl; apply f_equal2 with (f := fall) ; trivial.
     apply IHT with (X := S X).
 Qed.
 
-(** The following function substitutes the type variable number v
-    by newt inside t.                                              *)
-(** It is assumed that v is removed from the environment stack
-    and, as always, it is assumed that v does not appear in newt.  *)
+(** The following function substitutes the type variable number [v]
+    by [newt] inside [t].                                             *)
+(** It is assumed that [v] is removed from the environment stack
+    and, as always, it is assumed that [v] does not appear in [newt]. *)
 Fixpoint tsubst (t:typ) (v:nat) (newt:typ) : typ := 
   match t with
-    | vart l => (*several cases*)
-      if eq_nat_dec v l then
-        newt (*That's the variable to substitue*)
-      else if le_gt_dec l v then (*That's a variable before the target variable*) 
+    | vart l => (**r several cases*)
+      if eq_nat_dec v l then (**r That's the variable to substitue*)
+        newt
+      else if le_gt_dec l v then (**r That's a variable before the target variable*) 
              vart l
-           else (* That's a free variable, but we have a hole (we removed the variable)
-                 * so we need to garbage collect the name of this variable. *)
+           else (**r That's a free variable, but we have a hole (we removed the variable)
+                     so we need to garbage collect the name of this variable. *)
              vart (l-1)               
     | arrow t1 t2 => arrow (tsubst t1 v newt) (tsubst t2 v newt)
     | fall rank sp => fall rank (tsubst sp (1 + v) (tshift newt 0)) 
   end.
 
-Lemma tsubst_lemma_1 :
+(** The following lemma was inspired by Vouillon also we changed
+    the proof a lot. It will be useful in the next section.      *)
+Lemma tsubst_lemma :
   forall (T T' : typ) (X Y : nat),
     (tshift (tsubst T X T') (X + Y)) =
     (tsubst (tshift T (S (X + Y))) X (tshift T' (X + Y))).
@@ -78,47 +85,44 @@ Proof.
   induction T; intros T' X Y.
   + unfold tshift; unfold tsubst; fold tshift; fold tsubst.
     destruct (le_gt_dec (S (X + Y)) n).
-  - destruct (le_gt_dec n X); try omega.
-    destruct (le_gt_dec (1 + n) X); try omega.
-    destruct (eq_nat_dec X n); try omega.
-    destruct (eq_nat_dec X (1 + n)); try omega.
-    simpl.
-    destruct (le_gt_dec (X + Y) (n - 1)); try apply f_equal; omega.
-  - destruct (le_gt_dec n X);
-    destruct (eq_nat_dec X n) eqn:eq; auto;
-    simpl;
-    apply f_equal.
-    * destruct (le_gt_dec (X + Y) n); trivial.
-      omega.
-    * destruct (le_gt_dec (X + Y) (n - 1)); trivial.
-      omega.
-    + simpl; apply f_equal2 with (f := arrow); trivial.
-    + simpl; apply f_equal2 with (f := fall); trivial.
-      rewrite <- (plus_O_n (X+Y)) at 3.
-      rewrite <- (tshift_lemma_1 T' 0 (X + Y)).
-      rewrite plus_O_n.
-      apply (IHT _ (S X)).
+    - destruct (le_gt_dec n X); try omega.
+      destruct (le_gt_dec (1 + n) X); try omega.
+      destruct (eq_nat_dec X n); try omega.
+      destruct (eq_nat_dec X (1 + n)); try omega.
+      simpl.
+      destruct (le_gt_dec (X + Y) (n - 1)); try apply f_equal; omega.
+    - destruct (le_gt_dec n X);
+      destruct (eq_nat_dec X n) eqn:eq; auto;
+      simpl;
+      apply f_equal.
+      * destruct (le_gt_dec (X + Y) n); trivial.
+        omega.
+      * destruct (le_gt_dec (X + Y) (n - 1)); trivial.
+        omega.
+  + simpl; apply f_equal2 with (f := arrow); trivial.
+  + simpl; apply f_equal2 with (f := fall); trivial.
+    rewrite <- (plus_O_n (X+Y)) at 3.
+    rewrite <- (tshift_lemma T' 0 (X + Y)).
+    rewrite plus_O_n.
+    apply (IHT _ (S X)).
 Qed.
 
-(** Question 2 : Terms *)
+(** *** Question 2: Terms *)
 
 Inductive term :=
-| var : nat -> term
-(* The latter nat is the de Brujin index of the term variable. *)
-| abs : typ -> term -> term
-(* The latter typ is the type of the term which is abstracted. *)
+| var : nat -> term (**r maps a de Bruijn index to a term variable. *)
+| abs : typ -> term -> term (**r [typ] is the type of the term which is abstracted. *)
 | app : term -> term -> term
-| dept : nat -> term -> term
-(* The latter nat is the kind of the type which is abstracted. *)
+| dept : nat -> term -> term (**r [nat] is the kind of the type which is abstracted. *)
 | applt: term -> typ -> term.
 
 (** The following function shifts the free term variables
-    by one within the term t.                             *)
-(** v is the number of bounded variables
-    - ie number of lambda abstractions - in t.            *)
+    by one within the term [t].                           *)
+(** [v] is the number of bounded variables
+    - ie number of lambda abstractions around [t].        *)
 Fixpoint shift (t:term) (v:nat) : term :=
   match t with
-    | var i   =>  var (if le_gt_dec v i then 1 + i else i  )
+    | var i   =>  var (if le_gt_dec v i then 1 + i else i)
     | abs tp trm  => abs tp (shift trm (1 + v)) 
     | app trm1 trm2  => app (shift trm1 v) (shift trm2 v)
     | dept i trm => dept i (shift trm v) 
@@ -126,9 +130,9 @@ Fixpoint shift (t:term) (v:nat) : term :=
   end.
 
 (** The following function shifts the free type variables
-    by one within the term t.                             *)
-(** v is the number of bounded variables
-    - ie number of type abstractions - in t.              *)
+    by one within the term [t].                           *)
+(** [v] is the number of bounded variables
+    - ie number of type abstractions around [t].          *)
 Fixpoint shift_typ (t:term) (v:nat) : term :=
   match t with
     | var i   => var i
@@ -138,86 +142,84 @@ Fixpoint shift_typ (t:term) (v:nat) : term :=
     | applt trm tp =>  applt (shift_typ trm v) (tshift tp v)
   end.
 
-(** The following function substitutes the type variable number v
-    by newt inside t.                                             *)
-(** It is assumed that v is removed from the environment stack
-    and, as always, it is assumed that v does not appear in newt. *)
+(** The following function substitutes the type variable number [v]
+    by [newt] inside [t].                                             *)
+(** It is assumed that [v] is removed from the environment stack
+    and, as always, it is assumed that [v] does not appear in [newt]. *)
 Fixpoint subst_typ (trm:term) (v:nat) (newt:typ) := 
   match trm with
     | var l => var l 
     | abs tp trm => abs (tsubst tp v newt) (subst_typ trm v newt)
     | app trm1 trm2 => app (subst_typ trm1 v newt) (subst_typ trm2 v newt)
-    | dept i trm => dept i (subst_typ trm (1 + v) (tshift newt 0))
-    (*We need to bound FTV correctly, so we shift each time we cross a forall*)
+    | dept i trm => dept i (subst_typ trm (1 + v) (tshift newt 0)) (**r We need to bound FTV correctly, so we shift each time we cross a forall*)
     | applt trm tp => applt (subst_typ trm v newt) (tsubst tp v newt)
   end.
 
-(** The following function substitutes the term variable number v
-    by newt inside t.                                             *)
-(** It is assumed that v is removed from the environment stack
-    and, as always, it is assumed that v does not appear in newt. *)
+(** The following function substitutes the term variable number [v]
+    by [newt] inside [t].                                             *)
+(** It is assumed that [v] is removed from the environment stack
+    and, as always, it is assumed that [v] does not appear in [newt]. *)
 Fixpoint subst (trm:term) (v:nat) (newt:term) :=
   match trm with
     | var l =>
       if eq_nat_dec l v then newt
-      else if le_gt_dec l v then (*That's a variable before the target variable*) 
+      else if le_gt_dec l v then (**r That's a variable before the target variable*) 
              var l
-           else (* That's a free variable, but we have a hole (we removed the variable)
-                 * so we need to garbage collect the name of this variable. *)
+           else (**r That's a free variable, but we have a hole (we removed the variable)
+                     so we need to garbage collect the name of this variable. *)
              var (l-1)
     | abs tp trm => abs tp (subst trm (1 + v) (shift newt 0))
     | app trm1 trm2 => app (subst trm1 v newt) (subst trm2 v newt)
-    | dept i trm => dept i (subst trm v (shift_typ newt 0))
-    (* We need to shift FTV inside newt, to bound FTV correctly under new forallT *)
+    | dept i trm => dept i (subst trm v (shift_typ newt 0)) (**r We need to shift FTV inside newt, to bound FTV correctly under new forallT *)
     | applt trm tp => applt (subst trm v newt) tp
   end.
 
-(** Question 3 : Environments *)
-
-Require Import List.
-Import ListNotations.
+(** *** Question 3: Environments *)
 
 (** We use an array indexed by de Bruinj indexes - a stack -.    *)
 (** It can contain two sorts of info: the type of a term variable
     or the kind of a type variable.                              *)
 Inductive env :=
 | empty : env
-| v_typ : nat -> env -> env
-(* The latter nat is a kind. *)
+| v_typ : nat -> env -> env (**r This [nat] is a kind. *)
 | v : typ -> env -> env.
 
+(** A bit of monadic programming. It will be very useful to state
+    some lemmas. (Inspired by Vouillon)                           *)
 Definition map_under_option (A B : Set) (f: A -> B) (x: option A):=
   match x with 
     | Some x => Some (f x)
     | None => None
   end.
 
-(** The following function is used to get the type of the term variable
-    of index i in the environment e. *)
+(** The following function is used to get the type of
+    the term variable of index [i] in the environment [e]. *)
+(** This is a partial function returning an option.        *)
 Fixpoint get_typ e (i:nat) :=
   match e with
-    | empty => None               
-    | v_typ k tl => map_under_option _ _ (fun y=> tshift y 0) (get_typ tl i)                                        
+    | empty => None
+    | v_typ k tl => map_under_option _ _ (fun y => tshift y 0) (get_typ tl i)                                        
     | v t tl => match i with
                   | 0 => Some t
                   | S x => get_typ tl x
                 end
   end.
 
-(** The following function is used to get the kind of the type variable
-    of index i in the environment e. *)
+(** The following function is used to get the kind of
+    the type variable of index [i] in the environment [e]. *)
+(** This is a partial function returning an option.        *)
 Fixpoint get_kind e (i:nat) :=
   match e with
     | empty => None
-    | v_typ k tl => (match i with
+    | v_typ k tl => match i with
                        | 0 => Some k
                        | S x => get_kind tl x 
-                     end)
+                     end
     | v t tl => get_kind tl i
   end.
 
-(** Question 4 : kinding and typing predicates *)
-(** Question 5 : kind and type inference *)
+(** *** Question 4: kinding and typing predicates *)
+(** *** Question 5 : kind and type inference *)
 
 Fixpoint wf_typ (e : env) (T : typ) {struct T} : Prop :=
   match T with
@@ -226,17 +228,33 @@ Fixpoint wf_typ (e : env) (T : typ) {struct T} : Prop :=
     | fall k T2   => wf_typ (v_typ k e) T2 
   end.
 
-Local Open Scope bool_scope.
+(** This lemma will be useful in the next section.
+    (Inspired by Vouillon but the proof is ours.)  *)
+Lemma wf_typ_env_weaken :
+  forall (T : typ) (e e' : env),
+    (forall (X : nat), get_kind e' X = None -> get_kind e X = None) ->
+    wf_typ e T -> wf_typ e' T.
+Proof.
+  induction T; simpl; auto.
+  + intros e e' H [H1 H2].
+    split; eapply IHT1 || eapply IHT2; eauto.
+  + intros e e' H HT. 
+    apply IHT with (e := v_typ n e); trivial.
+    induction X; trivial.
+    simpl; firstorder.
+Qed.
 
+(** To each definition, we will associate an equivalent
+    boolean one which will be used for inference. *)
 Fixpoint wf_typ_bool (e : env) (T : typ) {struct T} : bool :=
   match T with
     | vart X      => match get_kind e X with | None => false | _ => true end
     | arrow T1 T2 => wf_typ_bool e T1 && wf_typ_bool e T2
     | fall k T2   => wf_typ_bool (v_typ k e) T2 
-  end
-.
+  end.
 
-Theorem wf_typ_equiv : forall T e, wf_typ_bool e T = true <-> wf_typ e T.
+(** And we will prove the equivalence each time. *)
+Lemma wf_typ_equiv : forall T e, wf_typ_bool e T = true <-> wf_typ e T.
 Proof.
   induction T; simpl; intros e.
   + destruct (get_kind e n); intuition.
@@ -246,6 +264,7 @@ Proof.
   + apply IHT; assumption.
 Qed.
 
+(** What it means for an environment to be well-formed. *)
 Fixpoint wf_env (e : env) : Prop :=
   match e with
     | empty     => True
@@ -260,7 +279,7 @@ Fixpoint wf_env_bool (e : env) : bool :=
     | v_typ T e => wf_env_bool e
   end.
 
-Theorem wf_env_equiv : forall e, wf_env_bool e = true <-> wf_env e.
+Lemma wf_env_equiv : forall e, wf_env_bool e = true <-> wf_env e.
 Proof.
   induction e; simpl.
   + intuition.
@@ -283,9 +302,9 @@ Inductive kinding (e : env) : typ -> nat -> Prop :=
                    kinding e (arrow tp1 tp2) (max p q)
 | kinded_fall : forall k1 tp1 p,
                   kinding (v_typ k1 e) tp1 p ->
-                  kinding e (fall k1 tp1) (1 + max p k1)
-.
+                  kinding e (fall k1 tp1) (1 + max p k1).
 
+(** This lemma will be useful in the next section. *)
 Lemma kinding_wf_typ : forall e tp k, kinding e tp k -> wf_typ e tp.
 Proof.
   induction 1; simpl in *; intuition.
@@ -294,7 +313,7 @@ Proof.
 Qed.
 
 (** Kind inference *)
-(** This function computes the minimal kind for a type term *)
+(** This function computes the minimal kind for a type term. *)
 Fixpoint kind (e : env) (tp : typ) : (option nat) :=
   match tp with
     | vart X => if wf_env_bool e then get_kind e X else None
@@ -306,70 +325,64 @@ Fixpoint kind (e : env) (tp : typ) : (option nat) :=
                        | Some p => Some (1 + max p k1)
                        | None => None
                      end
-  end
-.
+  end.
 
-Theorem correctness_of_kind : forall tp e k, kind e tp = Some k -> kinding e tp k.
+(** One of the two main theorems for this question. *)
+Theorem correctness_of_kind :
+  forall tp e k, kind e tp = Some k -> kinding e tp k.
 Proof.
   induction tp; intros e k H; simpl in H.
   + apply kinded_var with (p := k).
-  - destruct (wf_env_bool e); trivial.
-    discriminate.
-  - destruct (wf_env_bool e); trivial.
-  - apply wf_env_equiv.
-    destruct (wf_env_bool e); trivial.
-    discriminate.
-    + specialize IHtp1 with (e := e).
-      specialize IHtp2 with (e := e).
-      destruct (kind e tp1) as [q1 | _]; try discriminate.
-      destruct (kind e tp2) as [q2 | _]; try discriminate.
-      inversion H as [h].
-      apply kinded_arrow.
-  - apply IHtp1; reflexivity.
-  - apply IHtp2; reflexivity.
-    + specialize IHtp with (e := (v_typ n e)).
-      destruct (kind (v_typ n e)) as [p | _]; try discriminate.
-      inversion H as [h].
-      apply kinded_fall.
-      apply IHtp; reflexivity.
+    - destruct (wf_env_bool e); trivial.
+      discriminate.
+    - destruct (wf_env_bool e); trivial.
+    - apply wf_env_equiv.
+      destruct (wf_env_bool e); trivial.
+      discriminate.
+  + specialize IHtp1 with (e := e).
+    specialize IHtp2 with (e := e).
+    destruct (kind e tp1) as [q1 | _]; try discriminate.
+    destruct (kind e tp2) as [q2 | _]; try discriminate.
+    inversion H as [h].
+    apply kinded_arrow; auto.
+  + specialize IHtp with (e := (v_typ n e)).
+    destruct (kind (v_typ n e)) as [p | _]; try discriminate.
+    inversion H as [h].
+    apply kinded_fall.
+    apply IHtp; reflexivity.
 Qed.
 
 (** This result was not required by the subject.
-    But at first we had understood it was, so here it is *)
+    But at first we had understood it was, so here it is. *)
 Theorem completeness_of_kind :
   forall tp e k, (kinding e tp k) -> (exists p, p<=k /\ kind e tp = Some p).
 Proof.
   induction tp; intros e k kding; inversion kding.
   + exists p.
-           intuition.
-           rewrite <- H.
-           simpl.
-           rewrite <- wf_env_equiv in H2.
-           rewrite H2.
-           rewrite H.
-           assumption.
-           + intuition.
-             simpl.
-             specialize IHtp1 with (e := e) (k := p).
-             specialize IHtp2 with (e := e) (k := q).
-             destruct (IHtp1 H1) as [p0 [h1 h2]].
-             destruct (IHtp2 H3) as [q0 [h3 h4]].
-             exists (max p0 q0).
-             split.
-           - apply Nat.max_le_compat; assumption.
-           - rewrite h2; rewrite h4; reflexivity.
-             + specialize IHtp with (e := (v_typ n e)) (k := p).
-               destruct (IHtp H2) as [p0 [h1 h2]].
-               exists (1 + max p0 n). 
-               split.
-               * simpl.
-                 apply le_n_S.
-                 apply Nat.max_le_compat_r.
-                 assumption.
-               * simpl.
-                 rewrite h2.
-                 reflexivity.
-Qed. 
+    intuition.
+    rewrite <- H.
+    simpl.
+    rewrite <- wf_env_equiv in H2.
+    rewrite H2.
+    rewrite H.
+    assumption.
+  + intuition.
+    simpl.
+    specialize IHtp1 with (e := e) (k := p).
+    specialize IHtp2 with (e := e) (k := q).
+    destruct (IHtp1 H1) as [p0 [h1 h2]].
+    destruct (IHtp2 H3) as [q0 [h3 h4]].
+    exists (max p0 q0).
+    split.
+    - apply Nat.max_le_compat; assumption.
+    - rewrite h2; rewrite h4; reflexivity.
+  + specialize IHtp with (e := (v_typ n e)) (k := p).
+    destruct (IHtp H2) as [p0 [h1 h2]].
+    exists (1 + max p0 n). 
+    split; simpl; try lia.
+    rewrite h2.
+    reflexivity.
+Qed.
 
 (** Typing predicate *)
 (** After Figure 6: Stratified System F Type-Checking Rules *)
@@ -391,9 +404,9 @@ Inductive typing : env -> term -> typ -> Prop :=
 | typed_applt : forall e (trm : term) (tp1 tp2 : typ) (k : nat),
                   typing e trm (fall k tp1) ->
                   kinding e tp2 k ->
-                  typing e (applt trm tp2) (tsubst tp1 0 tp2)
-.
+                  typing e (applt trm tp2) (tsubst tp1 0 tp2).
 
+(** This lemma will be useful in the next section. *)
 Lemma typing_wf_env : forall e trm tp, typing e trm tp -> wf_env e.
 Proof.
   induction 1; simpl in *; intuition.
@@ -408,10 +421,9 @@ Fixpoint eq_typ t1 t2 : bool :=
     | (Top.arrow t11 t12 , Top.arrow t21 t22) => andb (eq_typ t11 t21) (eq_typ t12 t22)
     | (fall k11 t12 , fall k22 t22) => andb (beq_nat k11 k22) (eq_typ t12 t22)
     | _ => false
-  end
-.
+  end.
 
-Theorem eq_typ_equiv: forall t1 t2, eq_typ t1 t2 = true <-> t1 = t2.
+Lemma eq_typ_equiv: forall t1 t2, eq_typ t1 t2 = true <-> t1 = t2.
 Proof.
   induction t1; split; destruct t2; simpl; intro H; try discriminate.
   + rewrite beq_nat_eq with (x := n) (y := n0); intuition.
@@ -426,23 +438,21 @@ Proof.
     reflexivity.
   + inversion H.
     apply andb_true_iff; split.
-  - specialize IHt1_1 with (t2 := t2_1); destruct IHt1_1 as [_ iht1].
-    pattern t2_1 at 1; rewrite <- H1.
-    intuition.
-  - specialize IHt1_2 with (t2 := t2_2); destruct IHt1_2 as [_ iht2].
-    pattern t2_2 at 1; rewrite <- H2.
-    intuition.
-    + apply andb_true_iff in H; destruct H as [H1 H2].
-      specialize IHt1 with (t2 := t2); destruct IHt1 as [iht1 _].
-      rewrite (iht1 H2).
-      rewrite beq_nat_eq with (x := n) (y := n0); intuition.
-    + inversion H.
-      apply andb_true_iff; split.
-  - symmetry; apply beq_nat_refl.
-  - specialize IHt1 with (t2 := t2); destruct IHt1 as [_ iht1].
-    rewrite H2 in iht1.
-    apply iht1.
-    reflexivity.
+    - specialize IHt1_1 with (t2 := t2_1); destruct IHt1_1 as [_ iht1].
+      pattern t2_1 at 1; rewrite <- H1.
+      intuition.
+    - specialize IHt1_2 with (t2 := t2_2); destruct IHt1_2 as [_ iht2].
+      pattern t2_2 at 1; rewrite <- H2.
+      intuition.
+  + apply andb_true_iff in H; destruct H as [H1 H2].
+    specialize IHt1 with (t2 := t2); destruct IHt1 as [iht1 _].
+    rewrite (iht1 H2).
+    rewrite beq_nat_eq with (x := n) (y := n0); intuition.
+  + inversion H.
+    apply andb_true_iff; split.
+    - symmetry; apply beq_nat_refl.
+    - specialize IHt1 with (t2 := t2); destruct IHt1 as [_ iht1].
+      rewrite H2 in iht1; auto.
 Qed.
 
 (** Type inference *)
@@ -450,7 +460,7 @@ Fixpoint type (e : env) (trm : term) {struct trm} : option typ :=
   match trm with
     | var x => if wf_env_bool e then get_typ e x else None
     | abs tp1 trm1 => 
-      match kind e tp1 with (*This match is not necessary but it is an historical artefact.*)
+      match kind e tp1 with (**r This match is not necessary but it is an historical artefact.*)
         | Some a =>
           match type (v tp1 e) trm1  with 
             | None => None 
@@ -481,71 +491,70 @@ Fixpoint type (e : env) (trm : term) {struct trm} : option typ :=
           end
         | _ => None
       end
-  end
-.
+  end.
 
+(** One of the two main theorems for this question. *)
 Theorem correctness_of_type :
   forall trm tp e, type e trm = Some tp -> typing e trm tp.
 Proof.
   induction trm; intros tp e typ; simpl in typ.
   + apply (typed_var). 
-  - destruct (wf_env_bool e); trivial.
-    discriminate.
-  - apply wf_env_equiv.
-    destruct (wf_env_bool e); trivial.
-    discriminate.
-    + destruct (kind e t) eqn:eq1; try discriminate.
-      destruct (type (v t e) trm) eqn:eq; try discriminate.
-      inversion typ.
-      apply (typed_abs).
-      apply IHtrm; assumption.
-    + destruct (type e trm1) eqn:eq; try discriminate.
-      destruct (t) eqn:eq2; try discriminate.
-      destruct (type e trm2) eqn:eq1; try discriminate.
-      apply (typed_app e tp t0_1 trm1 trm2).
-  - apply (IHtrm1).
-    rewrite eq.
-    destruct (eq_typ t0_1 t0) eqn:eq3; try discriminate.
+    - destruct (wf_env_bool e); trivial.
+      discriminate.
+    - apply wf_env_equiv.
+      destruct (wf_env_bool e); trivial.
+      discriminate.
+  + destruct (kind e t) eqn:eq1; try discriminate.
+    destruct (type (v t e) trm) eqn:eq; try discriminate.
     inversion typ.
-    reflexivity.
-  - apply (IHtrm2).
-    destruct (eq_typ t0_1 t0) eqn:eq3; try discriminate.
-    rewrite eq1.
-    induction t0.
-    * specialize eq_typ_equiv with (t1 := t0_1) (t2 := vart n).
-      intros H; destruct H as [H1 H2].
-      rewrite H1; intuition.
-    * apply eq_typ_equiv in eq3.
-      rewrite eq3; reflexivity.
-    * apply eq_typ_equiv in eq3.
-      rewrite eq3; reflexivity.
-    + destruct (type (v_typ n e) trm) eqn:eq; try discriminate.
-      destruct tp; try discriminate.
+    apply typed_abs.
+    apply IHtrm; assumption.
+  + destruct (type e trm1) eqn:eq; try discriminate.
+    destruct (t) eqn:eq2; try discriminate.
+    destruct (type e trm2) eqn:eq1; try discriminate.
+    apply (typed_app e tp t0_1 trm1 trm2).
+    - apply (IHtrm1).
+      rewrite eq.
+      destruct (eq_typ t0_1 t0) eqn:eq3; try discriminate.
       inversion typ.
-      rewrite <- H0.
-      apply (typed_dept e n trm tp).
-      apply IHtrm. 
-      rewrite <- H1.
-      assumption.
-    + destruct (type e trm) eqn:eq; try discriminate.
-      destruct t0; try discriminate.
-      destruct (kind e t) eqn:eq1; try discriminate.
-      destruct (beq_nat n0 n) eqn:eq2; try discriminate.
-      inversion typ.
-      apply (typed_applt e trm t0 t n).
-  - apply IHtrm.
+      reflexivity.
+    - apply (IHtrm2).
+      destruct (eq_typ t0_1 t0) eqn:eq3; try discriminate.
+      rewrite eq1.
+      induction t0.
+      * specialize eq_typ_equiv with (t1 := t0_1) (t2 := vart n).
+        intros H; destruct H as [H1 H2].
+        rewrite H1; intuition.
+      * apply eq_typ_equiv in eq3.
+        rewrite eq3; reflexivity.
+      * apply eq_typ_equiv in eq3.
+        rewrite eq3; reflexivity.
+  + destruct (type (v_typ n e) trm) eqn:eq; try discriminate.
+    destruct tp; try discriminate.
+    inversion typ.
+    rewrite <- H0.
+    apply (typed_dept e n trm tp).
+    apply IHtrm. 
+    rewrite <- H1.
     assumption.
-  - apply correctness_of_kind.
-    rewrite eq1.
-    rewrite beq_nat_eq with (x := n0) (y := n); intuition.
+  + destruct (type e trm) eqn:eq; try discriminate.
+    destruct t0; try discriminate.
+    destruct (kind e t) eqn:eq1; try discriminate.
+    destruct (beq_nat n0 n) eqn:eq2; try discriminate.
+    inversion typ.
+    apply (typed_applt e trm t0 t n).
+    - apply IHtrm.
+      assumption.
+    - apply correctness_of_kind.
+      rewrite eq1.
+      rewrite beq_nat_eq with (x := n0) (y := n); intuition.
 Qed.
 
-(** 1.3 BASIC METATHEORY *)
+(** ** 1.3 Basic Metatheory *)
 
-(** Lemma 1.1 Cumulativity *)
+(** *** Lemma 1.1 (Cumulativity) *)
 
-Require Import Psatz.
-Lemma cumulativity :
+Theorem cumulativity :
   forall e t k k', kinding e t k -> k <= k' -> kinding e t k'.
 Proof.
   intros e t k k' kd; revert k'.
@@ -554,8 +563,8 @@ Proof.
     omega.
   + rewrite <- max_idempotent.
     apply (kinded_arrow e tp1 tp2 k' k');
-      (apply IHkd1 || apply IHkd2);
-      lia.
+    (apply IHkd1 || apply IHkd2);
+    lia.
   + assert (k' = 1 + max (k'-1) k1) as eq.
     lia.
     rewrite eq.
@@ -564,12 +573,12 @@ Proof.
     lia.
 Qed.
 
-(** 1.3.1 TYPE SUBSTITUTION *)
+(** ** 1.3.1 Type substitution *)
 
-(** Question 1 *)
+(** *** Question 1 *)
 
-(** insert_kind X e e' characterizes e' as being the extension of
-    e by a kinding declaration for variable X *)
+(** [insert_kind X e e'] characterizes [e'] as being the extension of
+    [e] by a kinding declaration for variable [X] *)
 Inductive insert_kind : nat -> env -> env -> Prop :=
 | insert_0 : forall k e,
                insert_kind 0 e (v_typ k e)
@@ -580,7 +589,7 @@ Inductive insert_kind : nat -> env -> env -> Prop :=
                      insert_kind n e e' ->
                      insert_kind (S n) (v_typ k e) (v_typ k e').
 
-(** Question 2 *)
+(** *** Question 2 *)
 
 Lemma insert_kind_get_kind :
   forall n e e' l,
@@ -589,25 +598,15 @@ Lemma insert_kind_get_kind :
 Proof.
   intros; revert l.
   induction H.
-  - simpl in *.
+  + simpl in *.
     destruct l; eauto.
-  - eauto.
-  - intuition. 
+  + eauto.
+  + intuition. 
     destruct l; trivial.
     specialize (IHinsert_kind l).
     simpl get_kind at 1.
     rewrite IHinsert_kind.
-    destruct (le_gt_dec n l); destruct (le_gt_dec (S n) (S l)). (**For now I can't find a better way to do that*)  
-    + eauto.
-    + assert( l<l).
-      omega.
-      apply lt_irrefl in H0.
-      contradiction H0.
-    + assert( n > n).
-      omega.
-      apply gt_irrefl in H0. 
-      contradiction H0.
-    + eauto.
+    destruct (le_gt_dec n l); destruct (le_gt_dec (S n) (S l)); eauto; omega.
 Qed.
 
 (** Well-formedness is invariant by weakening *)
@@ -616,26 +615,23 @@ Lemma insert_kind_wf_typ :
     insert_kind n e e' -> wf_typ e T -> wf_typ e' (tshift T n).
 Proof.
   induction T;
-  intros n' e e' a b.
-  - simpl in *. 
-    rewrite <-(insert_kind_get_kind n' e e' n).
-    eauto.
-    eauto.
-  - simpl in *. destruct b.  eauto.
-  - simpl in *. apply (IHT (S n') (v_typ n e) _ (insert_S_v_typ _ _ _ _ a) b).
+  intros n' e e' a b; simpl in *. 
+  + rewrite <- (insert_kind_get_kind n' e e' n); eauto.
+  + destruct b; eauto.
+  + exact (IHT (S n') (v_typ n e) _ (insert_S_v_typ _ _ _ _ a) b).
 Qed.
 
-Lemma insert_kind_wf_env :
+Theorem insert_kind_wf_env :
   forall (X : nat) (e e' : env),
     insert_kind X e e' -> wf_env e -> wf_env e'.
 Proof.
-  induction 1; simpl; auto. (*Induction on insert_kind*)
-  intros [T E];split; [apply (insert_kind_wf_typ _ _ e _); eauto | eauto].
+  induction 1; simpl; auto.
+  intros [T E].
+  split; try eapply insert_kind_wf_typ; eauto.
 Qed.
 
 (** Kinding is invariant by weakening *)
-
-Lemma insert_kind_kinding :
+Theorem insert_kind_kinding :
   forall T X e e' k,
     insert_kind X e e' ->
     kinding e T k ->
@@ -644,31 +640,28 @@ Proof.
   induction T; intros X e e' k H1 H2.
   + inversion H2.
     apply kinded_var with (p := p); trivial.
-  - rewrite <- H0.
-    symmetry.
-    apply insert_kind_get_kind.
-    assumption.
-  - eapply insert_kind_wf_env.
-    eassumption.
-    assumption.
-    + simpl.
-      rewrite <- max_idempotent.
-      apply kinded_arrow.
-  - apply IHT1 with (e := e); trivial.
-    inversion H2.
-    apply cumulativity with (k := p); trivial; lia.
-  - apply IHT2 with (e := e); trivial.
-    inversion H2.
-    apply cumulativity with (k := q); trivial; lia.
-    + simpl.
+    - rewrite <- H0.
+      symmetry.
+      apply insert_kind_get_kind.
+      assumption.
+    - eapply insert_kind_wf_env; eassumption.
+  + simpl.
+    rewrite <- max_idempotent.
+    apply kinded_arrow.
+    - apply IHT1 with (e := e); trivial.
       inversion H2.
-      apply kinded_fall.
-      apply IHT with (e := v_typ n e); trivial.
-      now apply insert_S_v_typ.
+      apply cumulativity with (k := p); trivial; lia.
+    - apply IHT2 with (e := e); trivial.
+      inversion H2.
+      apply cumulativity with (k := q); trivial; lia.
+  + simpl.
+    inversion H2.
+    apply kinded_fall.
+    apply IHT with (e := v_typ n e); trivial.
+    now apply insert_S_v_typ.
 Qed.
 
 (** Typing is invariant by weakening *)
-
 Lemma insert_kind_get_typ :
   forall (X : nat) (e e' : env),
     insert_kind X e e' ->
@@ -682,50 +675,50 @@ Proof.
     destruct (get_typ e y); trivial.
     simpl.
     apply f_equal.
-    exact (tshift_lemma_1 t 0 n).
+    exact (tshift_lemma t 0 n).
 Qed.
 
-Lemma insert_kind_typing :
+Theorem insert_kind_typing :
   forall (e e' : env) (X : nat) (trm : term) (tp : typ),
     insert_kind X e e' ->
     typing e trm tp ->
     typing e' (shift_typ trm X) (tshift tp X).
 Proof.
-  intros e e' X trm tp H1 H2; revert e' X H1; induction H2; intros e' X H1; simpl.
+  intros e e' X trm tp H1 H2;
+  revert e' X H1; induction H2;
+  intros e' X H1; simpl.
   + apply typed_var.
-  - rewrite <- insert_kind_get_typ with (X := X) (e := e); trivial.
-    rewrite H.
-    reflexivity.
-  - eapply insert_kind_wf_env; eauto.
-    + apply typed_abs.
-      apply IHtyping.
-      now apply insert_v.
-    + eapply typed_app.
-      now eapply IHtyping1.
-      now eapply IHtyping2.
-    + apply typed_dept.
-      apply IHtyping.
-      now apply insert_S_v_typ.
-    + rewrite (tsubst_lemma_1 _ _ 0 X).
-      eapply typed_applt; eauto.
-      simpl.
-      eapply insert_kind_kinding; eauto.
+    - rewrite <- insert_kind_get_typ with (X := X) (e := e); trivial.
+      rewrite H.
+      reflexivity.
+    - eapply insert_kind_wf_env; eauto.
+  + apply typed_abs.
+    apply IHtyping.
+    now apply insert_v.
+  + eapply typed_app.
+    - now eapply IHtyping1.
+    - now eapply IHtyping2.
+  + apply typed_dept.
+    apply IHtyping.
+    now apply insert_S_v_typ.
+  + rewrite (tsubst_lemma _ _ 0 X).
+    eapply typed_applt; eauto.
+    simpl.
+    eapply insert_kind_kinding; eauto.
 Qed.
 
-(** Question 3 *)
+(** *** Question 3 *)
 
 Inductive env_subst : nat -> typ -> env -> env -> Prop := 
-| subst_Svtyp: (*under the constructors*)
+| subst_Svtyp: (**r under the constructors*)
     forall e e' n k T,
-      (*wf_typ e' T ->*)
       env_subst n T e e' ->
       env_subst (S n) (tshift T 0) (v_typ k e) (v_typ k e')   
-| subst_SV: (*Substitute from the end to the beginning*)
+| subst_SV: (**r Substitute from the end to the beginning*)
     forall e e' n T tp,
-      (*wf_typ e' T ->*)
       env_subst n T e e' ->
       env_subst n T (v tp e) (v (tsubst tp n T) e')
-| substv: (*We need to substitue in e*)
+| substv: (**r We need to substitue in [e]*)
     forall e k T,
       wf_typ e T ->
       env_subst 0 T (v_typ k e) e.
@@ -742,26 +735,11 @@ Proof.
   apply insert_0.
 Qed.
 
-Lemma wf_typ_env_weaken :
-  forall (T : typ) (e e' : env),
-    (forall (X : nat), get_kind e' X = None -> get_kind e X = None) ->
-    wf_typ e T -> wf_typ e' T.
-Proof.
-  induction T; simpl; auto.
-  + intros e e' H [H1 H2].
-    split; eapply IHT1 || eapply IHT2; eauto.
-  + intros e e' H HT. 
-    apply IHT with (e := v_typ n e); trivial.
-    induction X; trivial.
-    simpl; firstorder.
-Qed.
-
-Lemma wf_typ_weakening_var :
+Lemma wf_typ_weak_strength_var :
   forall (e : env) (T1 T2 : typ),
-    wf_typ e T2 -> wf_typ (v T1 e) T2.
+    wf_typ e T2 <-> wf_typ (v T1 e) T2.
 Proof.
-  intros.
-  apply wf_typ_env_weaken with (e:= e); trivial.
+  split; apply wf_typ_env_weaken; trivial.
 Qed.
 
 Lemma get_typ_wf :
@@ -774,11 +752,13 @@ Proof.
     inversion H0.
     apply wf_typ_weakening_v_typ.
     eauto.
-  + apply wf_typ_weakening_var.
+  + apply wf_typ_weak_strength_var.
     destruct n; eauto.
     inversion H0 as [h0]; rewrite <- h0; auto.
 Qed.
 
+(** The following lemmas are deeply inspired by Vouillon
+    even if the proof is ours alone.                     *)
 Lemma env_subst_get_bound_lt :
   forall (X X' : nat) (e e' : env) (T : typ),
     (env_subst X' T e e') ->
@@ -819,7 +799,7 @@ Proof.
   - rewrite e0 in H; clear e0 X H1; revert H H0.
     induction 1; simpl; intuition.
     * now apply wf_typ_weakening_v_typ.
-    * now apply wf_typ_weakening_var.
+    * now apply wf_typ_weak_strength_var.
   - destruct (le_gt_dec n X); simpl.
     * erewrite env_subst_get_bound_lt; eauto.
       omega.
@@ -849,7 +829,8 @@ Proof.
   - eapply typing_wf_env; eauto.
 Qed.
 
-Lemma env_subst_wf_env :
+(** Well-formedness is invariant by [env_subst] *)
+Theorem env_subst_wf_env :
   forall X T e e',
     env_subst X T e e' ->
     wf_env e ->
@@ -859,176 +840,9 @@ Proof.
   eapply env_subst_wf_typ; eauto.
 Qed.
 
-(** Section 1.3.2 Term substitution *)
+(** ** 1.3.2 Term substitution *)
 
-(** TODO : move stuff here *)
-
-(**Partie 2*)
-
-(**A relation on (term x term) is term -> term -> Prop. Let define 
-our reduction relation with an inductive predicate.*)
-
-(**For now we don't care about well-formedness, it will come
-later*)
-(**Parallel reduction. I didn't find a better, automatic way. Nothin about congruence relations
-in the lib. It's intuition driven, so to check*)
-
-Require Import Relation_Definitions.
-
-
-Inductive oneStep : relation term :=
-| redTyp : forall phi n t, oneStep (applt (dept n t) phi) (subst_typ t 0 phi) (**TO check, I think there is a mistake*)
-| redTerm : forall (phi:typ) t (t':term), oneStep (Top.app (abs phi t) t') (subst t' 0  t)
-| redUnderAbs : forall phi t t', oneStep t t' -> oneStep (abs phi t) (abs phi t')
-| redUnderAbst : forall k t t', oneStep t t' -> oneStep (dept k t) (dept k t')
-(*We can do one parallelApp or two AppLeft AppRight. It's equivalent, but the second solution is
-easier for the proofs*)
-| parallelApp : forall t t' s s', oneStep t t' -> oneStep s s' -> oneStep (Top.app t s) (Top.app t' s')
-| redUnderAppt : forall t t' phi, oneStep t t' -> oneStep (applt t phi) (applt t' phi)
-| id : forall t, oneStep t t. (*TODO This is a choice, we could regret it later*)
-
-Require Import Relation_Operators.
-
-Definition reduction (t:term) (t':term) : Prop :=
-  clos_trans term oneStep t t'.
-
-(*We could probably factorize the following proofs*)
-Lemma congruAbs : forall t t' phi, reduction t t' -> reduction (abs phi t) (abs phi t').
-Proof.
-  intuition.
-  induction H.
-  - assert(oneStep (abs phi x) (abs phi y)). apply redUnderAbs; apply H.
-    apply t_step; apply H0.
-  - apply t_trans with (y:= abs phi y); firstorder.
-Qed.
-
-Lemma congruTypAbs : forall t t' k, reduction t t' -> reduction (dept k t) (dept k t').
-Proof.
-  intuition.
-  induction H.
-  - assert(oneStep (dept k x) (dept k y)). apply redUnderAbst; apply H.
-    apply t_step; apply H0.
-  - apply t_trans with (y:= dept k y); firstorder.
-Qed.
-
-Lemma congruTApp : forall t t' phi, reduction t t' -> reduction (applt t phi) (applt t' phi).
-Proof.
-  intuition.
-  induction H.
-  - assert(oneStep (applt x phi) (applt y phi)). apply redUnderAppt; apply H.
-    apply t_step; apply H0.
-  - apply t_trans with (y:= applt y phi); firstorder.
-Qed.
-
-(*We split in two lemmas, then we will merge the lemmas*)
-Lemma congruAppL : forall t t' s, reduction t t' -> reduction (Top.app t s) (Top.app t' s).
-Proof.
-  intuition.
-  induction H.
-  -  assert(oneStep (Top.app x s) (Top.app y s)). apply parallelApp; firstorder.
-     apply id; firstorder.
-     apply t_step; firstorder.
-  - apply t_trans with (y:=Top.app y s); firstorder.
-Qed.
-
-Lemma congruAppR : forall t t' s, reduction t t' -> reduction (Top.app s t) (Top.app s t').
-Proof.
-  intuition.
-  induction H.
-  -  assert(oneStep (Top.app s x) (Top.app s y)). apply parallelApp; firstorder.
-     apply id; firstorder.
-     apply t_step; firstorder.
-  - apply t_trans with (y:=Top.app s y); firstorder.
-Qed.
-
-Lemma congruApp : forall t t' s s', reduction t t' -> reduction s s' -> reduction (Top.app t s) (Top.app t' s').
-Proof.
-  intuition.
-  apply t_trans with (y:= Top.app t s').
-  apply congruAppR.
-  apply H0.
-  apply congruAppL.
-  apply H.
-Qed.
-
-(**Question 3*)
-(**System F is type erasing*)
-Inductive normal : term -> Prop :=
-| directlyNeutral: forall t, neutral t -> normal t
-| absNorm :  forall v phi, normal v -> normal (abs phi v) 
-| absTNorm : forall v k, normal v -> normal (dept k v) 
-with neutral : term -> Prop :=
-     | nV: forall n, neutral (var n)
-     | nApplt: forall phi t, neutral t -> neutral (applt t phi)
-     | nApp: forall t t', neutral t -> normal t' -> neutral (Top.app t t').
-
-
-(*Un terme neutre est un temre qui n'est pas une abstraction.*)
-
-
-Lemma normalPreservation : forall t n phi, (normal t -> normal (subst_typ t n phi)) /\ (neutral t -> neutral (subst_typ t n phi)). 
-Proof.
-  intros t.
-  induction t; intros nn phi.
-  - firstorder.
-  - simpl in *.
-    split.
-    intro.
-    apply absNorm.
-    apply IHt.
-    inversion H.
-    inversion H0.
-    apply H1.
-    intro.
-    inversion H.
-  - simpl in *.
-    split.
-    + intro.
-      apply directlyNeutral.
-      apply nApp.
-      inversion H.
-      inversion H0.
-      firstorder.
-      firstorder.
-      inversion H.  
-      apply IHt2.
-      inversion H.
-      inversion H0.
-      inversion H4.
-      easy.
-    + intro.
-      apply nApp;
-        inversion H.
-      apply IHt1.
-      apply H2.
-      apply IHt2.
-      apply H3.
-  - firstorder.
-    simpl in *.
-    apply absTNorm.
-    apply IHt.
-    inversion H.  
-    simpl in *.
-    inversion H0.
-    apply H1.
-    inversion H.
-  - firstorder.
-    simpl in *.
-    apply directlyNeutral.
-    apply nApplt.
-    apply IHt.
-    inversion H.
-    inversion H0.
-    apply H3.
-    simpl in *.
-    apply nApplt.
-    apply IHt.
-    inversion H.
-    apply H1.
-Qed.
-
-
-Fixpoint remove_var (x:nat) (e:env) {struct e}: env :=
+Fixpoint remove_var (x:nat) (e:env) {struct e} : env :=
   match e with
     | empty => empty
     | v_typ k e => v_typ k (remove_var x e)
@@ -1038,33 +852,23 @@ Fixpoint remove_var (x:nat) (e:env) {struct e}: env :=
                end
   end.
 
-Lemma get_typ_wk : forall e x y, x < y -> get_typ e x = get_typ (remove_var y e) x.
+Lemma get_typ_wk :
+  forall e x y, x < y -> get_typ e x = get_typ (remove_var y e) x.
 Proof.
-  induction e.
-  - eauto.
-  - firstorder.
-    simpl in *.
-    rewrite (IHe x y).
-    reflexivity.
-    apply H.
-  - intros x y H.
-    induction y.
-    * inversion H.
-    * induction x. 
-    +eauto. 
-    +apply IHe; omega.
+  induction e; intuition.
+  + simpl in *.
+    rewrite (IHe x y); trivial.
+  + induction y.
+    - inversion H.
+    - induction x. 
+      * eauto. 
+      * apply IHe; omega.
 Qed.
 
-Lemma wf_typ_strengthening_var :
-  forall (e : env) (T U : typ),
-    wf_typ (v T e ) U -> wf_typ e U.
+Lemma get_remove :
+  forall e n x , S x > n -> get_typ (remove_var n e) x = get_typ e (S x).
 Proof.
-  intros e T U H; apply wf_typ_env_weaken with (2 := H); simpl; trivial.
-Qed.
-
-Lemma get_remove : forall e n x , S x > n -> get_typ (remove_var n e) (x) = get_typ e (S x).
-Proof.
-  induction e;induction n; induction x; trivial;firstorder.
+  induction e; induction n; induction x; firstorder.
   - simpl.
     rewrite <- (IHe n 0).
     reflexivity.
@@ -1077,26 +881,29 @@ Proof.
   - omega.
 Qed.
 
-Lemma get_remove_2 : forall e x  n , x < n ->get_typ e  x = get_typ (remove_var n e) x .
+Lemma get_remove_2 :
+  forall e x  n , x < n -> get_typ e  x = get_typ (remove_var n e) x .
 Proof.
   induction e; trivial; intros x' n' H.
   - induction n'.
     * inversion H.
     * clear IHn'.
-      induction n; simpl;trivial.  rewrite (IHe x' (S n')). trivial. omega.
+      induction n; simpl; trivial.
+      rewrite (IHe x' (S n')); trivial; omega.
   - simpl.
-    induction x'; induction n'; trivial.
-    * omega.
-    * omega.
-    * firstorder.
+    induction x'; induction n'; firstorder; omega.
 Qed. 
 
-Lemma get_kind_remove : forall e x x', get_kind e x = get_kind (remove_var x' e) x.
+Lemma get_kind_remove :
+  forall e x x', get_kind e x = get_kind (remove_var x' e) x.
 Proof.
   induction e.
   * induction x'; simpl; trivial.
-  * induction x; trivial. intros. simpl in *. apply IHe.
-  * induction x'; intros; simpl;  trivial.
+  * induction x; trivial.
+    intros.
+    simpl in *.
+    auto.
+  * induction x'; intros; simpl; trivial.
 Qed.
 
 Lemma wf_typ_add : forall t e n, wf_typ (remove_var n e) t -> wf_typ e t.
@@ -1107,239 +914,270 @@ Proof.
     apply H.
 Qed.
 
-Lemma kinding_remove: forall u e n  W , wf_env e -> kinding (remove_var n e) u W -> kinding e u W.
+Lemma kinding_remove:
+  forall u e n  W ,
+  wf_env e -> kinding (remove_var n e) u W -> kinding e u W.
 Proof.
-  induction u.
-  -intuition.
-   inversion H0.
-   apply (kinded_var _ _ _ p ).
-   rewrite (get_kind_remove _ _ n0).
-   apply H2.
-   apply H3.
-   apply H.
-  - intuition.
-    inversion H0.
-    apply kinded_arrow.
-    apply (IHu1 e n _).
-    apply H.
-    apply H3.
-    apply (IHu2 e n _).
-    apply H.
-    apply H5.
-  -intuition.
-   inversion H0.
-   apply kinded_fall.
-   apply (IHu _ n0 _).
-   simpl.
-   apply H.
-   simpl.
-   apply H4.
+  induction u; intuition; inversion H0.
+  + eapply kinded_var; eauto.
+    erewrite get_kind_remove; eauto.
+  + apply kinded_arrow; firstorder.
+  + apply kinded_fall; firstorder.
 Qed.
 
-(**To shift the first n variables is the same that to remove the n first variable of the
-environment*)
-Lemma typ_shift_remove: forall e u W n, wf_env e -> typing (remove_var n e) u W -> typing e (shift u n) W.
+(** To shift the first [n] variables in [u] is the same as
+    to remove the first [n] variables from [e] *)
+Lemma typ_shift_remove:
+  forall (e : env) (u : term) (W : typ) (n : nat),
+  wf_env e -> typing (remove_var n e) u W -> typing e (shift u n) W.
 Proof.
   intuition.
   cut(exists e', e'= remove_var n e). (*Ce n'est pas comme assert! la coupure est ici nécessaire*)
-  - intros. destruct H1. rewrite <- H1 in H0.
-    generalize n e H1 H. clear n e H H1.
-    induction H0.
-    * firstorder; apply typed_var. 
+  - intros.
+    destruct H1.
+    rewrite <- H1 in H0.
+    revert n e H1 H; induction H0; firstorder; simpl.
+    * apply typed_var.
       rewrite H1 in H.
       simpl in *.
-      case (le_gt_dec n x).
-    + intros. rewrite <- (get_remove _ n). apply H. omega.
-    + intros. rewrite (get_remove_2 e0 x n). apply H.
-      omega.
-    + apply H2.
-      * intros. simpl.
-        apply typed_abs.
-        apply IHtyping.
-        rewrite H1.
-        trivial.  
-        simpl.
-        firstorder.
-        assert(wf_env (v tp1 e)).
-        apply (typing_wf_env (v tp1 e) trm1 tp2).
-        apply H0.
-        rewrite H1 in H2.
-        simpl in H2.
-        apply (wf_typ_add tp1 e0 n).
-        apply H2.
-      * intuition. simpl. apply (typed_app _ _ _ _ _ (IHtyping1 _ _ H1 H) (IHtyping2 _ _ H1 H)).
-      * intuition; simpl. 
-        apply typed_dept.
-        apply IHtyping.
-        rewrite H1.
-        trivial.
-        simpl.
-        apply H.
-      * intuition; simpl.
-        apply (typed_applt _ _ _ _ k).
-        apply IHtyping.
-        apply H1.
-        apply H2.
-        apply (kinding_remove _ _ n _ ).
-        apply H2.
-        rewrite <- H1.
-        apply H.
+      destruct (le_gt_dec n x).
+      + erewrite <- get_remove; eauto; omega.
+      + erewrite get_remove_2; eauto; omega.
+      + apply H2.
+    * apply typed_abs.
+      apply IHtyping.
+      now rewrite H1.
+      simpl.
+      firstorder.
+      specialize typing_wf_env with (e := v tp1 e) (trm := trm1) (tp := tp2); firstorder.
+      apply wf_typ_add with (n := n).
+      now rewrite <- H1.
+    * eapply typed_app; eauto.
+    * apply typed_dept.
+      apply IHtyping.
+      now rewrite H1.
+      simpl.
+      exact H.
+    * eapply typed_applt; eauto.
+      eapply kinding_remove with (n := n); eauto.
+      now rewrite <- H1.
   - exists (remove_var n e); trivial.
 Qed.
 
-Lemma wf_typ_remove: forall t e n,wf_typ e t -> wf_typ (remove_var n e) t.
+(** Well-formedness is invariant by [remove_var] *)
+Lemma wf_typ_remove:
+  forall t e n, wf_typ e t -> wf_typ (remove_var n e) t.
 Proof.
-  induction t;firstorder.
-  - simpl.
-    simpl in H.
-    rewrite <- get_kind_remove.
-    apply H.
+  induction t; firstorder; simpl in *.
+  now rewrite <- get_kind_remove.
 Qed.
 
-
-Lemma wf_env_remove: forall n e, wf_env e -> wf_env (remove_var n e).
+Theorem wf_env_remove: forall n e, wf_env e -> wf_env (remove_var n e).
 Proof.
-  induction n.
-  - induction e; firstorder. 
-  - induction e; firstorder.
-    apply wf_typ_remove.
-    apply H.
+  induction n; induction e; firstorder. 
+  now apply wf_typ_remove.
 Qed.
 
-Lemma kind_remove : forall tp2 e k n', wf_env e -> kinding e tp2 k -> kinding (remove_var n' e) tp2 k.
+(** Kinding is invariant by [remove_var]. *)
+Lemma kind_remove :
+  forall tp2 e k n',
+  wf_env e -> kinding e tp2 k -> kinding (remove_var n' e) tp2 k.
 Proof.
-  induction tp2; trivial; firstorder.
-  - inversion H0. 
-    apply (kinded_var _ _ _ p).
-    rewrite <- H2.
-    symmetry.
-    apply get_kind_remove.
-    apply H3.
-    apply wf_env_remove.
-    exact H4.
-  -inversion H0.
-   apply (kinded_arrow).
-   firstorder.
-   firstorder.
-  - inversion H0.
-    apply kinded_fall.    
-    firstorder.
+  induction tp2; firstorder; inversion H0. 
+  + eapply kinded_var; eauto.
+    - rewrite <- H2.
+      symmetry.
+      apply get_kind_remove.
+    - apply wf_env_remove; assumption.
+  + apply kinded_arrow; firstorder.
+  + apply kinded_fall; firstorder.
 Qed.
 
-(**From Vouillon*)
+(** Inspired by Vouillon. *)
 Lemma typing_weakening_var :
   forall (e : env) (t : term) (U V : typ),
     wf_typ e V -> typing e t U -> typing (v V e ) (shift t 0) U.
 Proof.
-  intros e t U V H1 H2; apply (typ_shift_remove (v V e));
-  simpl; trivial; split; trivial. 
-  apply (typing_wf_env e t U); firstorder.
+  intros.
+  apply typ_shift_remove; trivial.
+  simpl; firstorder.
+  eapply typing_wf_env; eauto.
 Qed.
 
-Lemma typing_weakening_bound_ind :
-  forall (e e' : env) (X : nat) (t : term) (U : typ),
-    insert_kind X e e' ->
-    typing e t U -> typing e' (shift_typ  t X) (tshift U X).
+Lemma typing_remove_vtyp:
+  forall e u W kl,
+  wf_typ e W ->
+  typing e u W ->
+  typing (v_typ kl e) (shift_typ u 0) (tshift W 0).
 Proof.
-  intros e e' n t U H1 H2; generalize n e' H1; clear n e' H1;
-  induction H2; intros n1 e' H1; simpl.
-  - apply typed_var.
-    + rewrite <-insert_kind_get_typ with (1:= H1). rewrite H; trivial. 
-    + exact (insert_kind_wf_env _ _ _ H1 H0).
-      
-  - apply typed_abs. apply IHtyping. apply insert_v. trivial.
-  - assert (H2 := (IHtyping1 _ _ H1)); assert (H3 := (IHtyping2 _ _ H1));
-    exact (typed_app _ _ _ _ _ H2 H3).
-  - apply typed_dept; apply IHtyping. apply insert_S_v_typ.
-    apply H1.
-  - rewrite (tsubst_lemma_1 _ _ 0 n1).
-    apply (typed_applt _ _ _ _ k) .
-    apply IHtyping.
-    apply H1.
-    simpl.
-    apply (insert_kind_kinding _ _ e _ _).
-    apply H1.
-    apply H.
-Qed.
-
-
-Lemma typing_remove_vtyp: forall e u W kl,  wf_typ e W -> typing e u W -> typing (v_typ kl e) (shift_typ u 0) (tshift W 0). (**The good way is to generalize slightly, saying that e' is e with et new kind somewhere*)
-Proof.
-  intros e t U V H1 H2; apply typing_weakening_bound_ind with (2 := H2).
+  (**r The good way is to generalize slightly, saying that e' is e with et new kind somewhere*)
+  intros.
+  eapply insert_kind_typing; eauto.
   apply insert_0.
 Qed.
 
-
-Lemma subst_preserves_typing :
+Theorem subst_preserves_typing :
   forall (e : env) (x : nat) (t u : term) (V W : typ),
     typing e t V -> 
     typing (remove_var x e) u W -> get_typ e x = Some W ->
     typing (remove_var x e) (subst t x u) V.
 Proof.
-  intros e n t u V W H ; generalize n u W; clear n u W;
-  induction H; intros n' u W H1 E1.
-  - simpl. case_eq (eq_nat_dec x n').
-    +  intros H2 _.
-       rewrite H2 in *.
-       rewrite E1 in H.
-       inversion H.
-       rewrite <- H4.
-       apply H1.
-    + intros H2 _. 
-      case (le_gt_dec).
-      * intro H3.
-        apply typed_var.
-        assert (x<n'). omega.
-        rewrite <- (get_typ_wk e x n').
-        apply H.
-        apply H4.
-        apply (typing_wf_env (remove_var n' e) u W).
-        apply H1.
-      * intro H3.
-        apply typed_var.
-        assert  (x = S (x-1)).
+  intros e n t u V W H ; revert n u W; induction H; intros n' u W H1 E1; simpl.
+  - destruct (eq_nat_dec x n') as [H2 | H2].
+    + rewrite H2 in H; rewrite E1 in H.
+      inversion H.
+      now rewrite <- H4.
+    + case le_gt_dec; intros H3; apply typed_var;
+      try (eapply typing_wf_env; eauto).
+      * rewrite <- (get_typ_wk e x n'); auto; omega.
+      * rewrite get_remove; try omega.
+        assert (S (x - 1) = x) as eq.
         omega.
-        rewrite H4.
-        simpl.
-        rewrite get_remove.
-        assert(x-1-0=x-1).
-        omega.
-        rewrite H5.
-        assert( S (x - 1)=x).
-        omega.
-        rewrite H6.
-        apply H.
-        omega.
-        apply (typing_wf_env (remove_var n' e) u W).
-        apply H1.
-  - simpl. apply typed_abs.
-    apply (IHtyping  (S n') (shift u 0) W). trivial.
+        rewrite eq; assumption.
+  - apply typed_abs.
+    apply (IHtyping  (S n') (shift u 0) W); trivial.
     simpl.
     assert(wf_env (v tp1 e)).
-    apply (typing_wf_env _ trm1 tp2).
-    apply H.
+    eapply typing_wf_env; eauto.
     simpl in H0.
-    destruct H0.
-    assert (H3 := wf_typ_remove _ _ n' H0 ).    
-    apply typing_weakening_var;trivial.
-    simpl.
-    apply E1.
-  - exact (typed_app _ _ _ _ _ (IHtyping1 _ u W H1 E1) (IHtyping2 _ u W H1 E1)).
-  - simpl; apply typed_dept. apply (IHtyping n' (shift_typ u 0) (tshift W 0)).
-    * simpl. apply typing_remove_vtyp;firstorder.
-      apply (typing_wf_typ _ u).
-      apply H1.
-    * simpl; rewrite E1; trivial.
-  - simpl. apply typed_applt with (1 := (IHtyping _ u W H1 E1)). 
+    destruct H0.   
+    apply typing_weakening_var; trivial.
+    eapply wf_typ_remove; eauto.
+  - eapply typed_app; eauto.
+  - apply typed_dept.
+    apply (IHtyping n' (shift_typ u 0) (tshift W 0)); simpl.
+    * apply typing_remove_vtyp; firstorder.
+      eapply typing_wf_typ; eauto.
+    * rewrite E1; trivial.
+  - eapply typed_applt; eauto.
     apply kind_remove.
-    apply (typing_wf_env e trm (fall k tp1)).
-    apply H.
-    apply H0.
+    eapply typing_wf_env; eauto.
+    exact H0.
 Qed.
 
-
-Lemma typing_weakening_var_ind :
+Theorem typing_weakening_var_ind :
   forall (e : env) (x : nat) (t : term) (U : typ),
     wf_env e -> typing (remove_var x e) t U -> typing e (shift t x) U.
+Abort.
 
-(** Do the same for kinding weakening and preservation*)
+(** TODO: the same for kinding weakening and preservation*)
+
+(** TODO: Regularity and Narrowing *)
+
+(** ** 2 Reduction and Normal Terms *)
+
+(** *** Question 1 *)
+
+(** A relation on [term * term] is [term -> term -> Prop].           *)
+(** Let's define our reduction relation with an inductive predicate. *)
+
+(** For now we don't care about well-formedness, it will come later. *)
+(** Parallel reduction.                                              *)
+(** I didn't find a better, automatic way.
+    Nothing about congruence relations in the lib.                   *)
+
+Inductive oneStep : relation term :=
+| redTyp : forall phi n t, oneStep (applt (dept n t) phi) (subst_typ t 0 phi) (*TO check, I think there is a mistake*)
+| redTerm : forall (phi:typ) t (t':term), oneStep (Top.app (abs phi t) t') (subst t' 0  t)
+| redUnderAbs : forall phi t t', oneStep t t' -> oneStep (abs phi t) (abs phi t')
+| redUnderAbst : forall k t t', oneStep t t' -> oneStep (dept k t) (dept k t') (**r We can do one parallelApp or two AppLeft AppRight. It's equivalent, but the second solution is easier for the proofs*)
+| parallelApp : forall t t' s s', oneStep t t' -> oneStep s s' -> oneStep (Top.app t s) (Top.app t' s')
+| redUnderAppt : forall t t' phi, oneStep t t' -> oneStep (applt t phi) (applt t' phi)
+| id : forall t, oneStep t t. (*TODO This is a choice, we could regret it later*)
+
+Definition reduction (t:term) (t':term) : Prop :=
+  clos_trans term oneStep t t'.
+
+(** *** Question 2 *)
+
+(** We could probably factorize the following proofs. *)
+Lemma congruAbs :
+  forall t t' phi,
+  reduction t t' -> reduction (abs phi t) (abs phi t').
+Proof.
+  induction 1.
+  - apply t_step.
+    now apply redUnderAbs.
+  - eapply t_trans; eauto.
+Qed.
+
+Lemma congruTypAbs :
+  forall t t' k,
+  reduction t t' -> reduction (dept k t) (dept k t').
+Proof.
+  induction 1.
+  - apply t_step.
+    now apply redUnderAbst.
+  - eapply t_trans; eauto.
+Qed.
+
+Lemma congruTApp :
+  forall t t' phi,
+  reduction t t' -> reduction (applt t phi) (applt t' phi).
+Proof.
+  induction 1.
+  - apply t_step.
+    now apply redUnderAppt.
+  - eapply t_trans; eauto.
+Qed.
+
+(*We split in two lemmas, then we will merge the lemmas*)
+Lemma congruAppL :
+  forall t t' s,
+  reduction t t' -> reduction (Top.app t s) (Top.app t' s).
+Proof.
+  induction 1.
+  - apply t_step.
+    apply parallelApp; trivial.
+    apply id.
+  - eapply t_trans; eauto.
+Qed.
+
+Lemma congruAppR :
+  forall t t' s,
+  reduction t t' -> reduction (Top.app s t) (Top.app s t').
+Proof.
+  induction 1.
+  - apply t_step.
+    apply parallelApp; trivial.
+    apply id.
+  - eapply t_trans; eauto.
+Qed.
+
+Lemma congruApp :
+  forall t t' s s',
+  reduction t t' ->
+  reduction s s' ->
+  reduction (Top.app t s) (Top.app t' s').
+Proof.
+  intros.
+  eapply t_trans; apply congruAppR || apply congruAppL; eauto.
+Qed.
+
+(** *** Question 3 *)
+
+(**  System F is type erasing*)
+Inductive normal : term -> Prop :=
+| directlyNeutral: forall t, neutral t -> normal t
+| absNorm :  forall v phi, normal v -> normal (abs phi v) 
+| absTNorm : forall v k, normal v -> normal (dept k v) 
+with neutral : term -> Prop := (**r A neutral term is one that is not an abstraction. *)
+     | nV: forall n, neutral (var n)
+     | nApplt: forall phi t, neutral t -> neutral (applt t phi)
+     | nApp: forall t t', neutral t -> normal t' -> neutral (Top.app t t').
+
+Theorem normalPreservation :
+  forall t n phi,
+  (normal t -> normal (subst_typ t n phi)) /\
+  (neutral t -> neutral (subst_typ t n phi)). 
+Proof.
+  induction t; firstorder; simpl in *; inversion H; inversion H0.
+  + apply absNorm; firstorder.
+  + apply directlyNeutral.
+    apply nApp; firstorder.
+  + apply nApp; firstorder.
+  + apply absTNorm; firstorder.
+  + apply directlyNeutral.
+    apply nApplt; firstorder.
+  + apply nApplt; firstorder.
+Qed.
